proof: defined constraint_gen cg_fun
Typo fix

Typo fix

cogent/isa/CogentInference.thy
@@ -32,7 +32,6 @@ type_synonym name = string
 type_synonym index = nat
 
 datatype type = TVar index
-              | TVarBang index
               | TFun type type
               | TPrim prim_type
               | TProduct type type
@@ -42,19 +41,24 @@ datatype type = TVar index
 datatype lit = LBool bool
              | LNat nat
 
+fun subst_ty :: "type list \<Rightarrow> type \<Rightarrow> type" where
+  "subst_ty \<delta> (TVar i)       = \<delta> ! i"
+| "subst_ty \<delta> (TFun a b)     = TFun (subst_ty \<delta> a) (subst_ty \<delta> b)"
+| "subst_ty \<delta> (TPrim p)      = TPrim p"
+| "subst_ty \<delta> (TProduct t u) = TProduct (subst_ty \<delta> t) (subst_ty \<delta> u)"
+| "subst_ty \<delta> (TUnit)        = TUnit"
+| "subst_ty \<delta> (TUnknown i)   = TUnknown i"
 
-datatype 'f expr = Var index
-                 | AFun 'f  "type list"
-                 | Fun "'f expr" "type list"
-                 | Prim prim_op "'f expr list"
-                 | App "'f expr" "'f expr"
-                 | Unit
-                 | Lit lit
-                 | SLit string
-                 | Cast num_type "'f expr"
-                 | Let "'f expr" "'f expr"
-                 | If "'f expr" "'f expr" "'f expr"
-                 | Sig "'f expr" type
+
+
+fun max_type_var :: "type \<Rightarrow> nat" where
+  "max_type_var (TVar i)       = i"
+| "max_type_var (TFun a b)     = max (max_type_var a) (max_type_var b)"
+| "max_type_var (TPrim p)      = 0"
+| "max_type_var (TProduct t u) = max (max_type_var t) (max_type_var u)"
+| "max_type_var (TUnit)        = 0"
+| "max_type_var (TUnknown i)   = 0"
+
 
 datatype constraint =
   CtConj constraint constraint
@@ -66,20 +70,50 @@ datatype constraint =
   | CtShare type
   | CtDrop type
 
+fun map_types_ct :: "(type \<Rightarrow> type) \<Rightarrow> constraint \<Rightarrow> constraint" where
+  "map_types_ct f (CtConj a b)    = CtConj (map_types_ct f a) (map_types_ct f b)"
+| "map_types_ct f (CtIBound l t)  = CtIBound l (f t)"
+| "map_types_ct f (CtEq a b)      = CtEq (f a) (f b)"
+| "map_types_ct f (CtSub a b)     = CtSub (f a) (f b)"
+| "map_types_ct f (CtTop)         = CtTop"
+| "map_types_ct f (CtBot)         = CtBot"
+| "map_types_ct f (CtShare t)     = CtShare (f t)"
+| "map_types_ct f (CtDrop t)      = CtDrop (f t)"
+
+definition subst_ct :: "type list \<Rightarrow> constraint \<Rightarrow> constraint" where
+  "subst_ct \<delta> \<equiv> map_types_ct (subst_ty \<delta>)"
+
+
+locale type_infer =
+  fixes type_of :: "'fnname \<Rightarrow> constraint \<times> type"
+begin
+
+datatype 'f expr = Var index
+                 | TypeApp 'f "type list"
+                 | Prim prim_op "'f expr list"
+                 | App "'f expr" "'f expr"
+                 | Unit
+                 | Lit lit
+                 | SLit string
+                 | Cast num_type "'f expr"
+                 | Let "'f expr" "'f expr"
+                 | If "'f expr" "'f expr" "'f expr"
+                 | Sig "'f expr" type
+
 type_synonym cg_ctx = "(type \<times> nat) list"
 
-inductive alg_ctx_jn :: "cg_ctx \<Rightarrow> nat \<Rightarrow> cg_ctx \<Rightarrow> nat \<Rightarrow> cg_ctx \<Rightarrow> nat \<Rightarrow> constraint \<Rightarrow> bool"
-            ("_,_ \<Join> _,_ \<leadsto> _,_ | _" [30,0,0,0,0,0,30] 60) where
-  "\<lbrakk> \<And>i. i < length G
-   ; length G = length G'
-   ; fst (G!i) = fst (G'!i)
-   ; m!i = max (snd (G!i)) (snd (G'!i)) 
-   ; G2!i = (fst (G!i), (m!i))
-   ; if (snd (G!i)) = (snd (G'!i)) then (C!i) = CtTop else (C!i) = CtDrop (fst (G!i))
+inductive alg_ctx_jn :: "cg_ctx \<Rightarrow> cg_ctx \<Rightarrow> cg_ctx \<Rightarrow> constraint \<Rightarrow> bool"
+            ("_ \<Join> _ \<leadsto> _ | _" [30,0,0,30] 60) where
+  alg_ctx_jn: 
+  "\<lbrakk> map fst G = map fst G'
+   ; list_all3 (\<lambda>m g g'. m = max (snd g) (snd g')) m G G'
+   ; list_all3 (\<lambda>g2 g m. g2 = (fst g, m)) G2 G M
+   ; C = List.map2 (\<lambda>g g'. if (snd g) = (snd g') then CtTop else CtDrop (fst g)) G G'
    ; C2 = foldr CtConj C CtTop
-   \<rbrakk> \<Longrightarrow> G,n \<Join> G',n' \<leadsto> G2,n2 | C2"
+   \<rbrakk> \<Longrightarrow> G \<Join> G' \<leadsto> G2 | C2"
 
-inductive constraint_gen :: "cg_ctx \<Rightarrow> nat \<Rightarrow> 'f expr \<Rightarrow> type \<Rightarrow> cg_ctx \<Rightarrow> nat \<Rightarrow> constraint \<Rightarrow> bool"
+
+inductive constraint_gen :: "cg_ctx \<Rightarrow> nat \<Rightarrow> 'fnname expr \<Rightarrow> type \<Rightarrow> cg_ctx \<Rightarrow> nat \<Rightarrow> constraint \<Rightarrow> bool"
             ("_,_ \<turnstile> _ : _ \<leadsto> _,_ | _" [30,0,0,0,0,0,30] 60) where
   cg_var1: 
   "\<lbrakk> G!i = (\<rho>,0) 
@@ -99,13 +133,13 @@ inductive constraint_gen :: "cg_ctx \<Rightarrow> nat \<Rightarrow> 'f expr \<Ri
 | cg_app:
   "\<lbrakk> \<alpha> = TUnknown (Suc n1)
    ; G1,(Suc n1) \<turnstile> e1 : TFun \<alpha> \<tau> \<leadsto> G2,n2 | C1
-   ; G2,n2' \<turnstile> e2 : \<alpha> \<leadsto> G3,n3 | C2
+   ; G2,n2 \<turnstile> e2 : \<alpha> \<leadsto> G3,n3 | C2
    ; C3 = CtConj C1 C2
    \<rbrakk> \<Longrightarrow> G1,n1 \<turnstile> App e1 e2 : \<tau> \<leadsto> G3,n3 | C3"
 | cg_let:
   "\<lbrakk> \<alpha> = TUnknown (Suc n1)
    ; G1,(Suc n1) \<turnstile> e1 : \<alpha> \<leadsto> G2,n2 | C1
-   ; ((\<alpha>, 0) # G2),n2' \<turnstile> e2 : \<tau> \<leadsto> ((\<alpha>, m) # G3),n3 | C2 
+   ; ((\<alpha>, 0) # G2),n2 \<turnstile> e2 : \<tau> \<leadsto> ((\<alpha>, m) # G3),n3 | C2 
    ; if m = 0 then C3 = CtDrop \<alpha> else C3 = CtTop
    ; C4 = CtConj (CtConj C1 C2) C3
    \<rbrakk> \<Longrightarrow> G1,n1 \<turnstile> Let e1 e2 : \<tau> \<leadsto> G3,n3 | C4"
@@ -114,29 +148,83 @@ inductive constraint_gen :: "cg_ctx \<Rightarrow> nat \<Rightarrow> 'f expr \<Ri
 | cg_ilit:
   "C = CtIBound (LNat m) \<tau> \<Longrightarrow> G,n \<turnstile> Lit (LNat m) : \<tau> \<leadsto> G,n | C"
 | cg_if:
-  "\<lbrakk> G1,n1 \<turnstile> e1 : (TPrim Bool) \<leadsto> G2,2 | C1
-   ; G2,n2' \<turnstile> e2 : \<tau> \<leadsto> G3,n3 | C2
-   ; G2,n2'' \<turnstile> e3 : \<tau> \<leadsto> G3',n3' | C3
-   ; G3,n3'' \<Join> G3',n3''' \<leadsto> G4,n4 | C4 
+  "\<lbrakk> G1,n1 \<turnstile> e1 : (TPrim Bool) \<leadsto> G2,n2 | C1
+   ; G2,n2 \<turnstile> e2 : \<tau> \<leadsto> G3,n3 | C2
+   ; G2,n3 \<turnstile> e3 : \<tau> \<leadsto> G3',n4 | C3
+   ; G3 \<Join> G3' \<leadsto> G4 | C4 
    ; C5 = CtConj (CtConj (CtConj C1 C2) C3) C4
    \<rbrakk> \<Longrightarrow> G1,n1 \<turnstile> If e1 e2 e3 : \<tau> \<leadsto> G4,n4 | C5"
 | cg_iop:
   "\<lbrakk> e \<in> {Prim (Plus nt), Prim (Minus nt), Prim (Times nt), Prim (Divides nt)}
    ; G1,n1 \<turnstile> e1 : \<tau> \<leadsto> G2,n2 | C1
-   ; G2,n2' \<turnstile> e2 : \<tau> \<leadsto> G3,n3 | C2
+   ; G2,n2 \<turnstile> e2 : \<tau> \<leadsto> G3,n3 | C2
    ; C5 = CtConj (CtConj (CtIBound (LNat 0) \<tau>) C1) C2
    \<rbrakk> \<Longrightarrow> G1,n1 \<turnstile> e [e1, e2] : \<tau> \<leadsto> G3,n3 | C5"
 | cg_cop:
   "\<lbrakk> \<alpha> = TUnknown (Suc n1)
    ; e \<in> {Prim (Eq (Num nt)), Prim (NEq (Num nt)), Prim (Lt nt), Prim (Gt nt), Prim (Le nt), Prim (Ge nt)}
    ; G1,(Suc n1) \<turnstile> e1 : \<alpha> \<leadsto> G2,n2 | C1
-   ; G2,n2' \<turnstile> e2 : \<alpha> \<leadsto> G3,n3 | C2
+   ; G2,n2 \<turnstile> e2 : \<alpha> \<leadsto> G3,n3 | C2
    ; C3 = CtConj (CtConj (CtConj (CtIBound (LNat 0) \<alpha>) (CtEq \<tau> (TPrim Bool))) C1) C2 
    \<rbrakk> \<Longrightarrow> G1,n1 \<turnstile> e [e1, e2] : \<tau> \<leadsto> G3,n3 | C3"
 | cg_bop:
   "\<lbrakk> e \<in> {Prim (BitAnd nt), Prim (BitOr nt)}
    ; G1,n1 \<turnstile> e1 : \<tau> \<leadsto> G2,n2 | C1
-   ; G2,n2' \<turnstile> e2 : \<tau> \<leadsto> G3,n3 | C2 
+   ; G2,n2 \<turnstile> e2 : \<tau> \<leadsto> G3,n3 | C2 
    ; C3 = CtConj (CtConj (CtEq \<tau> (TPrim Bool)) C1) C2
   \<rbrakk> \<Longrightarrow> G1,n1 \<turnstile> e [e1, e2] : \<tau> \<leadsto> G3,n3 | C3"
+| cg_tapp:
+  "\<lbrakk> (C, \<rho>) = type_of name
+   (* make fresh unknown \<beta>s for each variable past those we are substituting into the type *)
+   ; m = Suc (max_type_var \<rho>) - length ts
+   ; \<beta>s = map (TUnknown \<circ> (+) (Suc n1)) [0..<m]
+   ; \<rho>' = subst_ty (ts @ \<beta>s) \<rho>
+   ; C' = subst_ct (ts @ \<beta>s) C
+   ; C2 = CtConj (CtSub \<rho>' \<tau>) C'
+   ; n' = n + m
+   \<rbrakk> \<Longrightarrow> G,n \<turnstile> TypeApp name ts : \<tau> \<leadsto> G,n' | C2"
+
+lemma
+  assumes "G,n \<turnstile> e : \<tau> \<leadsto> G',n' | C"
+  shows "n \<ge> n'"
+  using assms
+proof (induct rule: constraint_gen.inducts)
+case (cg_var1 G i \<rho> G' C \<tau> n)
+  then show ?case sorry
+next
+  case (cg_var2 G i \<rho> n G' C \<tau>)
+  then show ?case sorry
+next
+  case (cg_sig G1 n1 e \<tau>' G2 n2 C C' \<tau>)
+  then show ?case sorry
+next
+  case (cg_app \<alpha> n1 G1 e1 \<tau> G2 n2 C1 e2 G3 n3 C2 C3)
+  then show ?case sorry
+next
+  case (cg_let \<alpha> n1 G1 e1 G2 n2 C1 e2 \<tau> m G3 n3 C2 C3 C4)
+  then show ?case sorry
+next
+  case (cg_blit C \<tau> G n l)
+  then show ?case sorry
+next
+  case (cg_ilit C m \<tau> G n)
+  then show ?case sorry
+next
+  case (cg_if G1 n1 e1 G2 n2 C1 e2 \<tau> G3 n3 C2 e3 G3' n4 C3 G4 C4 C5)
+  then show ?case sorry
+next
+  case (cg_iop e nt Divides G1 n1 e1 \<tau> G2 n2 C1 e2 G3 n3 C2 C5)
+  then show ?case sorry
+next
+  case (cg_cop \<alpha> n1 e nt G1 e1 G2 n2 C1 e2 G3 n3 C2 C3 \<tau>)
+  then show ?case sorry
+next
+  case (cg_bop e nt G1 n1 e1 \<tau> G2 n2 C1 e2 G3 n3 C2 C3)
+  then show ?case sorry
+next
+case (cg_tapp C \<rho> name m ts \<beta>s n1 \<rho>' C' C2 \<tau> n' n G)
+  then show ?case sorry
+qed
+
+end
 end                            
